fix & add Principia.Formula

Logic/Predicate/FirstOrder/Arith/Model.lean
@@ -13,14 +13,14 @@ namespace Semantics
 instance standardModel : Structure oRing ℕ where
   func := fun _ f =>
     match f with
-    | ORingFunc.zero => fun _ => 0
-    | ORingFunc.one  => fun _ => 1
-    | ORingFunc.add  => fun v => v 0 + v 1
-    | ORingFunc.mul  => fun v => v 0 * v 1
+    | ORing.Func.zero => fun _ => 0
+    | ORing.Func.one  => fun _ => 1
+    | ORing.Func.add  => fun v => v 0 + v 1
+    | ORing.Func.mul  => fun v => v 0 * v 1
   rel := fun _ r =>
     match r with
-    | ORingRel.eq => fun v => v 0 = v 1
-    | ORingRel.lt => fun v => v 0 < v 1
+    | ORing.Rel.eq => fun v => v 0 = v 1
+    | ORing.Rel.lt => fun v => v 0 < v 1
 
 instance : Structure.Eq oRing ℕ := ⟨by simp[standardModel]⟩
 
@@ -40,10 +40,10 @@ variable {μ : Type v} (e : Fin n → ℕ) (ε : μ → ℕ)
 @[simp] lemma mul_eq_mul : standardModel.func lang(*) ![x, y] = x * y := rfl
 
 @[simp] lemma numeral_eq_numeral (n : ℕ) :
-    Subterm.val standardModel e ε (Subterm.natLit oRing n) = n := by 
+    Subterm.val standardModel e ε (Subterm.numeral oRing n) = n := by
   induction' n with n ih
-  { simp[Subterm.natLit_zero] }
-  { cases' n with n <;> simp[Subterm.natLit_one, ←Nat.one_eq_succ_zero, Subterm.natLit_succ, Nat.succ_eq_add_one] at ih ⊢
+  { simp[Subterm.numeral_zero] }
+  { cases' n with n <;> simp[Subterm.numeral_one, ←Nat.one_eq_succ_zero, Subterm.numeral_succ, Nat.succ_eq_add_one] at ih ⊢
     simp[ih] }
 
 @[simp] lemma lt_eq_lt : standardModel.rel lang(<) ![x, y] ↔ x < y := of_eq rfl
@@ -52,7 +52,7 @@ variable {μ : Type v} (e : Fin n → ℕ) (ε : μ → ℕ)
     Subformula.Eval standardModel e ε “ᵀ!t ≤ ᵀ!u”  ↔ t.val standardModel e ε ≤ u.val standardModel e ε :=
   by simp[Subformula.le_eq, le_iff_eq_or_lt]
 
-theorem modelsTheoryPAminus : ℕ ⊧* Theory.PAminus oRing := by
+lemma modelsTheoryPAminusAux : ℕ ⊧* Theory.PAminus oRing := by
   intro σ h
   rcases h <;> simp[models_def]
   case addAssoc => intro l m n; exact add_assoc n m l
@@ -66,19 +66,8 @@ theorem modelsTheoryPAminus : ℕ ⊧* Theory.PAminus oRing := by
   case ltTrans => intro l m n; exact Nat.lt_trans
   case ltTri => intro n m; simp[or_assoc]; exact Nat.lt_trichotomy m n
 
-theorem modelsTheoryRobinson : ℕ ⊧* Theory.Robinson oRing := by
-  intro σ h
-  rcases h <;> simp[models_def]
-  case q₃ => intro x; cases x <;> simp
-  case q₅ => simp[add_assoc]
-  case q₇ => simp[mul_add]
-  case q₈ =>
-    intro x y
-    simp[Subformula.le_eq, Nat.lt_iff_add_one_le, le_iff_exists_add];
-    exact ⟨by rintro ⟨z, rfl⟩; exact ⟨z, by simp[add_comm]⟩, by rintro ⟨z, rfl⟩; exact ⟨z, by simp[add_comm]⟩⟩
-
-@[simp] theorem modelsRobinson : ℕ ⊧* Axiom.Robinson oRing := by
-  simp[Axiom.Robinson, modelsTheoryRobinson]
+theorem modelsTheoryPAminus : ℕ ⊧* Axiom.PAminus oRing := by
+  simp[Axiom.PAminus, modelsTheoryPAminusAux]
 
 lemma modelsSuccInd (σ : Subsentence oRing (k + 1)) : ℕ ⊧ (Arith.succInd σ) := by
   simp[succInd, models_iff, Matrix.constant_eq_singleton, Matrix.comp_vecCons', Subformula.eval_substs]
@@ -87,7 +76,7 @@ lemma modelsSuccInd (σ : Subsentence oRing (k + 1)) : ℕ ⊧ (Arith.succInd σ
   · exact hsucc x ih
 
 lemma modelsPeano : ℕ ⊧* Axiom.Peano oRing :=
-  by simp[Axiom.Peano, Axiom.Ind, Theory.IndScheme, modelsSuccInd]
+  by simp[Axiom.Peano, Axiom.Ind, Theory.IndScheme, modelsSuccInd, modelsTheoryPAminus]
 
 end standardModel
 
