Logic/Predicate/FirstOrder/Principia/Formula.lean
@@ -1,0 +1,281 @@
+import Logic.Predicate.FirstOrder.Principia.Term
+
+open Qq Lean Elab Meta Tactic
+
+-- Subformula normalization
+
+namespace LO
+
+namespace FirstOrder
+
+namespace Principia
+
+namespace lemmataFormula
+
+variable {L : Language.{u}} {μ : Type v} {n}
+
+open Subformula
+
+lemma rel_ext {k} (r : L.rel k) (v w : Fin k → Subterm L μ₁ n₁) (H : ∀ i, v i = w i) :
+    rel r v = rel r w := congr_arg _ (funext H)
+
+lemma nrel_ext {k} (r : L.rel k) (v w : Fin k → Subterm L μ₁ n₁) (H : ∀ i, v i = w i) :
+    nrel r v = nrel r w := congr_arg _ (funext H)
+
+lemma finitary_ext {k} (f : Finitary L k) (v w : Fin k → Subterm L μ n) (H : ∀ i, v i = w i) :
+    f.operator v = f.operator w := congr_arg _ (funext H)
+
+section Rew
+
+variable (ω : Rew L μ₁ n₁ μ₂ n₂)
+
+lemma rew_rel_eq_of_eq {k} (r : L.rel k) {v : Fin k → Subterm L μ₁ n₁} {v'} (h : ∀ i, ω (v i) = v' i) :
+    ω.hom (rel r v) = rel r v' :=
+  by simp[Rew.rel, Function.comp, h]
+
+lemma rew_nrel_eq_of_eq {k} (r : L.rel k) {v : Fin k → Subterm L μ₁ n₁} {v'} (h : ∀ i, ω (v i) = v' i) :
+    ω.hom (nrel r v) = nrel r v' :=
+  by simp[Rew.nrel, Function.comp, h]
+
+lemma rew_const_eq_of_eq (c : Const L) :
+    ω.hom (Operator.const c) = Operator.const c :=
+  Rew.hom_const ω c
+
+lemma rew_finitary_eq_of_eq {k} (f : Finitary L k) {v : Fin k → Subterm L μ₁ n₁} {v'} (h : ∀ i, ω (v i) = v' i) :
+    ω.hom (f.operator v) = f.operator v' :=
+  by simp[Rew.hom_operator, Function.comp, h]
+
+
+
+end Rew
+
+lemma shift_substs_eq_of_eq {t : SyntacticSubterm L k} {w : Fin k → SyntacticSubterm L n} {t' w'}
+  (ht : Rew.shift t = t') (hw : ∀ i, Rew.shift (w i) = w' i) :
+    Rew.shift (Rew.substs w t) = Rew.substs w' t' := by
+  simp[←ht, ←hw, ←Rew.comp_app, Rew.shift_comp_substs]
+  congr; funext i; simp[hw]
+
+lemma subst_bshift_0 (v : Fin 1 → Subterm L μ 0) (t : Subterm L μ 0) : Rew.substs v (Rew.bShift t) = t := by simp[Rew.comp]
+
+end lemmataFormula
+
+inductive DFormula (L : Q(Language.{u})) : ℕ → Type
+  | verum {n} : DFormula L n
+  | falsum {n} : DFormula L n
+  | rel {n arity : ℕ} : Q(($L).rel $arity) → (Fin arity → DTerm L n) → DFormula L n
+  | nrel {n arity : ℕ} : Q(($L).rel $arity) → (Fin arity → DTerm L n) → DFormula L n
+  | const {n} (c : Q(Subformula.Const.{u, 0} $L)) : DFormula L n
+  | finitary {n arity : ℕ} (f : Q(Subformula.Finitary.{u, 0} $L $arity)) : (Fin arity → DTerm L n) → DFormula L n
+  | and {n} : DFormula L n → DFormula L n → DFormula L n
+  | or  {n} : DFormula L n → DFormula L n → DFormula L n
+  | neg {n} : DFormula L n → DFormula L n
+  | imply {n} : DFormula L n → DFormula L n → DFormula L n
+  | iff {n} : DFormula L n → DFormula L n → DFormula L n
+  | all {n} : DFormula L (n + 1) → DFormula L n
+  | ex {n} : DFormula L (n + 1) → DFormula L n
+  | expr {n : ℕ} : Q(SyntacticSubformula $L $n) → DFormula L n
+
+namespace DFormula
+
+instance : Inhabited (DFormula L n) := ⟨verum⟩
+
+def toStr {L : Q(Language.{u})} {n : ℕ} : DFormula L n → String
+  | verum        => "⊤"
+  | falsum       => "⊥"
+  | rel _ v      => "rel " ++ "(" ++ (String.vecToStr fun i => (v i).toStr) ++ ")"
+  | nrel _ v     => "nrel " ++ "(" ++ (String.vecToStr fun i => (v i).toStr) ++ ")"
+  | const _      => "const"
+  | finitary _ v => "finitary " ++ "(" ++ (String.vecToStr fun i => (v i).toStr) ++ ")"
+  | and p q      => "(" ++ p.toStr ++ ") ∧ (" ++ q.toStr ++ ")"
+  | or p q       => "(" ++ p.toStr ++ ") ∨ (" ++ q.toStr ++ ")"
+  | neg p        => "¬(" ++ p.toStr ++ ")"
+  | imply p q    => "(" ++ p.toStr ++ ") → (" ++ q.toStr ++ ")"
+  | iff p q      => "(" ++ p.toStr ++ ") ↔ (" ++ q.toStr ++ ")"
+  | all p        => "∀[" ++ p.toStr ++ "]"
+  | ex p         => "∃[" ++ p.toStr ++ "]"
+  | expr _       => "expr"
+
+instance : Repr (DTerm L n) := ⟨fun t _ => DTerm.toStr t⟩
+
+instance : ToString (DTerm L n) := ⟨DTerm.toStr⟩
+
+@[reducible] def toExpr {L : Q(Language.{u})} {n : ℕ} :
+    DFormula L n → Q(SyntacticSubformula $L $n)
+  | verum        => q(⊤)
+  | falsum       => q(⊥)
+  | rel r v      =>
+    let w := Qq.vecFold q(SyntacticSubterm $L $n) (fun i => (v i).toExpr)
+    q(Subformula.rel $r $w)
+  | nrel r v     =>
+    let w := Qq.vecFold q(SyntacticSubterm $L $n) (fun i => (v i).toExpr)
+    q(Subformula.nrel $r $w)
+  | const c      => q(Subformula.Operator.const $c)
+  | finitary f v =>
+    let w := Qq.vecFold q(SyntacticSubterm $L $n) (fun i => (v i).toExpr)
+    q(Subformula.Operator.operator $f $w)
+  | and p q      => q($p.toExpr ⋏ $q.toExpr)
+  | or p q       => q($p.toExpr ⋎ $q.toExpr)
+  | neg p        => q(~$p.toExpr)
+  | imply p q    => q($p.toExpr ⟶ $q.toExpr)
+  | iff p q      => q($p.toExpr ⟷ $q.toExpr)
+  | all p        => q(∀' $p.toExpr)
+  | ex p         => q(∃' $p.toExpr)
+  | expr e       => e
+
+protected def isDefEq {L : Q(Language.{u})} {n} (p₁ p₂ : DFormula L n) : MetaM Bool :=
+  Lean.Meta.isDefEq p₁.toExpr p₂.toExpr
+
+partial def denote (L : Q(Language.{u})) (n : ℕ) : (p : Q(SyntacticSubformula $L $n)) → MetaM (DFormula L n)
+  | ~q(⊤) => pure verum
+  | ~q(⊥) => pure falsum
+  | ~q(Subformula.rel (arity := $arity) $r $v)  => do
+    let arity' : ℕ ← Denotation.denote arity
+    let v' ← vecUnfold q(SyntacticSubterm $L $n) arity' v
+    let v'' ← Matrix.getM fun i => DTerm.denote L n (v' i)
+    return rel r v''
+  | ~q(Subformula.nrel (arity := $arity) $r $v) => do
+    let arity' : ℕ ← Denotation.denote arity
+    let v' ← vecUnfold q(SyntacticSubterm $L $n) arity' v
+    let v'' ← Matrix.getM fun i => DTerm.denote L n (v' i)
+    return nrel r v''
+  | ~q(Subformula.Operator.const $c)                         => pure (const c)
+  | ~q(Subformula.Operator.operator (ι := Fin $arity) $r $v) => do
+    let arity' : ℕ ← Denotation.denote arity
+    let v' ← vecUnfold q(SyntacticSubterm $L $n) arity' v
+    let v'' ← Matrix.getM fun i => DTerm.denote L n (v' i)
+    return finitary r v''
+  | ~q($p ⋏ $q)  => return and (←denote L n p) (←denote L n q)
+  | ~q($p ⋎ $q)  => return or (←denote L n p) (←denote L n q)
+  | ~q(~$p)      => return neg (←denote L n p)
+  | ~q($p ⟶ $q) => return imply (←denote L n p) (←denote L n q)
+  | ~q($p ⟷ $q)  => return iff (←denote L n p) (←denote L n q)
+  | ~q(∀' $p)    => return all (←denote L (n + 1) p)
+  | ~q(∃' $p)    => return ex (←denote L (n + 1) p)
+  | ~q($p)       => return expr p
+
+instance (L : Q(Language.{u})) (n) : Denotation (DFormula L n) where
+  denote := denote L n
+  toExpr := toExpr
+
+structure DEq {L : Q(Language.{u})} {n : ℕ} (p₁ p₂ : DFormula L n) where
+  expr : Q($(p₁.toExpr) = $(p₂.toExpr))
+
+local infix:20 " ≡ " => DFormula.DEq
+
+namespace DEq
+
+variable {L : Q(Language.{u})} {n : ℕ}
+
+
+@[refl] protected def refl (p : DFormula L n) : p ≡ p := .mk q(rfl)
+
+@[symm] protected def symm {p₁ p₂ : DFormula L n} (h : p₁ ≡ p₂) : p₂ ≡ p₁ :=
+  .mk q(Eq.symm $h.expr)
+
+@[trans] protected def trans {p₁ p₂ p₃ : DFormula L n} (h₁ : p₁ ≡ p₂) (h₂ : p₂ ≡ p₃) : p₁ ≡ p₃ :=
+  .mk q(Eq.trans $h₁.expr $h₂.expr)
+
+def ofIsDefEq (p₁ p₂ : DFormula L n) : p₁ ≡ p₂ := ⟨(q(@rfl (SyntacticSubformula $L $n) $p₁.toExpr) : Expr)⟩
+
+def relExt {arity : ℕ} (r : Q(($L).rel $arity)) {v w : Fin arity → DTerm L n} (H : (i : Fin arity) → (v i).DEq (w i)) :
+    rel r v ≡ rel r w := by
+  let v' := Qq.vecFold q(SyntacticSubterm $L $n) (fun i => (v i).toExpr)
+  let w' := Qq.vecFold q(SyntacticSubterm $L $n) (fun i => (w i).toExpr)
+  let H : Q(∀ i, $v' i = $w' i) := vecFoldDep q(fun i => $v' i = $w' i) (fun i => (H i).expr)
+  let e : Q(Subformula.rel $r $v' = Subformula.rel $r $w') := q(lemmataFormula.rel_ext $r _ _ $H)
+  exact .mk e
+
+def nrelExt {arity : ℕ} (r : Q(($L).rel $arity)) {v w : Fin arity → DTerm L n} (H : (i : Fin arity) → (v i).DEq (w i)) :
+    nrel r v ≡ nrel r w := by
+  let v' := Qq.vecFold q(SyntacticSubterm $L $n) (fun i => (v i).toExpr)
+  let w' := Qq.vecFold q(SyntacticSubterm $L $n) (fun i => (w i).toExpr)
+  let H : Q(∀ i, $v' i = $w' i) := vecFoldDep q(fun i => $v' i = $w' i) (fun i => (H i).expr)
+  let e : Q(Subformula.nrel $r $v' = Subformula.nrel $r $w') := q(lemmataFormula.nrel_ext $r _ _ $H)
+  exact .mk e
+
+def finitaryExt {arity : ℕ}
+  (f : Q(Subformula.Finitary.{u, 0} $L $arity)) {v w : Fin arity → DTerm L n} (H : (i : Fin arity) → (v i).DEq (w i)) :
+    finitary f v ≡ finitary f w := by
+  let v' := Qq.vecFold q(SyntacticSubterm $L $n) (fun i => (v i).toExpr)
+  let w' := Qq.vecFold q(SyntacticSubterm $L $n) (fun i => (w i).toExpr)
+  let H : Q(∀ i, $v' i = $w' i) := vecFoldDep q(fun i => $v' i = $w' i) (fun i => (H i).expr)
+  let e : Q(($f).operator $v' = ($f).operator $w') := q(lemmataFormula.finitary_ext $f _ _ $H)
+  exact .mk e
+
+end DEq
+
+abbrev qrew (L : Q(Language.{u})) (n m: ℕ) (ω : Q(Rew $L ℕ $n ℕ $m)) : Q(SyntacticSubformula $L $n → SyntacticSubformula $L $m) := q(($ω).hom)
+
+abbrev qsubsts {L : Q(Language.{u})} {arity n : ℕ} (v : Fin arity → DTerm L n) :
+    Q(SyntacticSubformula $L $arity → SyntacticSubformula $L $n) :=
+  let v' := Qq.vecFold q(SyntacticSubterm $L $n) (fun i => (v i).toExpr)
+  qrew L arity n q(Rew.substs $v')
+
+abbrev qshift {L : Q(Language.{u})} {n : ℕ} : Q(SyntacticSubformula $L $n → SyntacticSubformula $L $n) :=
+  qrew L n n q(Rew.shift)
+
+abbrev qbShift {L : Q(Language.{u})} {n : ℕ} : Q(SyntacticSubformula $L $n → SyntacticSubformula $L ($n + 1)) :=
+  qrew L n (n + 1) q(Rew.bShift)
+
+abbrev qfix {L : Q(Language.{u})} {n : ℕ} : Q(SyntacticSubformula $L $n → SyntacticSubformula $L ($n + 1)) :=
+  qrew L n (n + 1) q(Rew.fix)
+
+abbrev qfree {L : Q(Language.{u})} {n : ℕ} : Q(SyntacticSubformula $L ($n + 1) → SyntacticSubformula $L $n) :=
+  qrew L (n + 1) n q(Rew.free)
+
+structure DEqFun {L : Q(Language.{u})} {n₁ n₂ : ℕ} (f : Q(SyntacticSubformula $L $n₁ → SyntacticSubformula $L $n₂))
+  (p₁ : DFormula L n₁) (p₂ : DFormula L n₂) where
+  expr : Q($f $(p₁.toExpr) = $(p₂.toExpr))
+
+local notation:25 p₁ " ≡[" f:25 "] " p₂:0 => DEqFun f p₁ p₂
+
+namespace DEqFun
+
+variable {L : Q(Language.{u})} {n : ℕ}
+
+def ofDEqFunOfDEq {n₁ n₂ : ℕ} {f : Q(SyntacticSubformula $L $n₁ → SyntacticSubformula $L $n₂)}
+  {p₁ : DFormula L n₁} {p₂ p₂' : DFormula L n₂} (df : p₁ ≡[f] p₂) (de : p₂ ≡ p₂') :
+    p₁ ≡[f] p₂' := ⟨q(Eq.trans $df.expr $de.expr)⟩
+
+def rewRel {arity n m : ℕ} (ω : Q(Rew $L ℕ $n ℕ $m)) (r : Q(($L).rel $arity))
+  {v : Fin arity → DTerm L n} {w : Fin arity → DTerm L m}
+  (H : ∀ i, DTerm.DEqFun (DTerm.qrew L n m ω) (v i) (w i)) : rel r v ≡[qrew L n m ω] rel r w := by
+  let v' := Qq.vecFold q(SyntacticSubterm $L $n) (fun i => (v i).toExpr)
+  let w' := Qq.vecFold q(SyntacticSubterm $L $m) (fun i => (w i).toExpr)
+  let H : Q(∀ i, $ω ($v' i) = $w' i) := vecFoldDep q(fun i => $ω ($v' i) = $w' i) (fun i => (H i).expr)
+  let e : Q(($ω).hom (Subformula.rel $r $v') = Subformula.rel $r $w') := q(lemmataFormula.rew_rel_eq_of_eq _ $r $H)
+  exact .mk e
+
+def rewNrel {arity n m : ℕ} (ω : Q(Rew $L ℕ $n ℕ $m)) (r : Q(($L).rel $arity))
+  {v : Fin arity → DTerm L n} {w : Fin arity → DTerm L m}
+  (H : ∀ i, DTerm.DEqFun (DTerm.qrew L n m ω) (v i) (w i)) : nrel r v ≡[qrew L n m ω] nrel r w := by
+  let v' := Qq.vecFold q(SyntacticSubterm $L $n) (fun i => (v i).toExpr)
+  let w' := Qq.vecFold q(SyntacticSubterm $L $m) (fun i => (w i).toExpr)
+  let H : Q(∀ i, $ω ($v' i) = $w' i) := vecFoldDep q(fun i => $ω ($v' i) = $w' i) (fun i => (H i).expr)
+  let e : Q(($ω).hom (Subformula.nrel $r $v') = Subformula.nrel $r $w') := q(lemmataFormula.rew_nrel_eq_of_eq _ $r $H)
+  exact .mk e
+
+def rewFinitary {arity n m : ℕ} (ω : Q(Rew $L ℕ $n ℕ $m))
+  (f : Q(Subformula.Finitary.{u, 0} $L $arity)) {v : Fin arity → DTerm L n} {w : Fin arity → DTerm L m}
+  (H : ∀ i, DTerm.DEqFun (DTerm.qrew L n m ω) (v i) (w i)) : finitary f v ≡[qrew L n m ω] finitary f w := by
+  let v' := Qq.vecFold q(SyntacticSubterm $L $n) (fun i => (v i).toExpr)
+  let w' := Qq.vecFold q(SyntacticSubterm $L $m) (fun i => (w i).toExpr)
+  let H : Q(∀ i, $ω ($v' i) = $w' i) := vecFoldDep q(fun i => $ω ($v' i) = $w' i) (fun i => (H i).expr)
+  let e : Q(($ω).hom (($f).operator $v') = ($f).operator $w') := q(lemmataFormula.rew_finitary_eq_of_eq _ $f $H)
+  exact .mk e
+
+def rewConst {n m : ℕ} (ω : Q(Rew $L ℕ $n ℕ $m))
+  (c : Q(Subformula.Const.{u, 0} $L)) : (const c : DFormula L n) ≡[qrew L n m ω] const c := by
+  let e : Q(($ω).hom (Subformula.Operator.const $c) = Subformula.Operator.const $c) := q(lemmataFormula.rew_const_eq_of_eq _ $c)
+  exact .mk e
+
+end DEqFun
+
+
+end DFormula
+
+end Principia
+
+end FirstOrder
+
+end LO
